src/fstar/FStar.Main.fst
@@ -202,6 +202,7 @@ let go _ =
 let lazy_chooser k i = match k with
     | FStar.Syntax.Syntax.BadLazy -> failwith "lazy chooser: got a BadLazy"
     | FStar.Syntax.Syntax.Lazy_bv         -> FStar.Reflection.Embeddings.unfold_lazy_bv          i
+    | FStar.Syntax.Syntax.Lazy_namedv     -> FStar.Reflection.Embeddings.unfold_lazy_namedv      i
     | FStar.Syntax.Syntax.Lazy_binder     -> FStar.Reflection.Embeddings.unfold_lazy_binder      i
     | FStar.Syntax.Syntax.Lazy_letbinding -> FStar.Reflection.Embeddings.unfold_lazy_letbinding  i
     | FStar.Syntax.Syntax.Lazy_optionstate -> FStar.Reflection.Embeddings.unfold_lazy_optionstate i
@@ -216,6 +217,7 @@ let lazy_chooser k i = match k with
     | FStar.Syntax.Syntax.Lazy_universe   -> FStar.Reflection.Embeddings.unfold_lazy_universe    i
     | FStar.Syntax.Syntax.Lazy_universe_uvar -> FStar.Syntax.Util.exp_string "((universe_uvar))"
     | FStar.Syntax.Syntax.Lazy_issue -> FStar.Syntax.Util.exp_string "((issue))"
+    | FStar.Syntax.Syntax.Lazy_ident -> FStar.Syntax.Util.exp_string "((ident??)"
 
 // This is called directly by the Javascript port (it doesn't call Main)
 let setup_hooks () =
